theories/Stlc/Persistence.v
@@ -43,7 +43,7 @@ Import World.notations.
 #[local] Set Implicit Arguments.
 
 Class Persistent (A : TYPE) : Type :=
-  persist : forall {Θ}, ⊧ A ̂→ Box Θ A.
+  persist : forall {Θ}, ⊧ A ⇢ Box Θ A.
 #[global] Arguments persist {_ _ _} [w] _ [_] _.
 
 #[export] Instance persist_ty : Persistent Ṫy :=
